
# $Date: 2011-05-28 11:36:37 -0400 (Sat, 28 May 2011) $
# $Revision: 30841 $
# $Author: oshani $

# The Respect My Privacy Vocabulary Definition
# author: tkang@mit.edu

@prefix rdf:  <http://www.w3.org/1999/02/22-rdf-syntax-ns#> .
@prefix rdfs: <http://www.w3.org/2000/01/rdf-schema#> .
@prefix owl: <http://www.w3.org/2002/07/owl#> .
@prefix vs: <http://www.w3.org/2003/06/sw-vocab-status/ns#> .
@prefix cc: <http://creativecommons.org/ns#> .
@prefix foaf: <http://xmlns.com/foaf/0.1/> .
@prefix : <http://dig.csail.mit.edu/2008/02/rmp/rmp-schema#> .


:restricts a rdfs:Property;
	rdfs:comment "Applies a restriction";
	rdfs:label "restricts";
	rdfs:range :Restriction.

:Restriction a rdfs:Class;
	rdfs:comment "A privacy restriction";
	rdfs:label "Privacy Restriction".

:No-Cookies a :Restriction;
        rdfs:comment "The no-cookies restriction is used in HTTPA.the server will not place any first-party or third-party cookies on the user's hard disk";
        rdfs:label "No Cookies".
		
:No-Third-Party-Cookies a :Restriction;
        rdfs:comment "The no-third-party-cookies restriction is used in HTTPA. The server will not place any third-party cookies on the user's hard disk.";
        rdfs:label "No Third-Party Cookies".

:No-User-Tracking a :Restriction;
        rdfs:comment "The no-user-tracking restriction is used in HTTPA. The server will place a cookie on to the user's hard disk, but this cookie will not in any way track the user behavior over time and report to a central ad network. It will only be used in website personalization.";
        rdfs:label "No User Tracking".

:No-Ownership-Transfer a :Restriction;
        rdfs:comment "The no-ownership-tranfer restriction is used in HTTPA. The ownership of the data item is with the data producer and it is non-transferable";
        rdfs:label "No Ownership Transfer".


:No-Commercial a :Restriction;
	rdfs:comment "The no-commercial restriction states that the owner of this profile does not want the information on this profile used for commercial purposes.";
	rdfs:label "No-Commercial".
	
:No-Depiction a :Restriction;
	rdfs:comment "The no-depiction restriction states that the owner of this profile does not want this profile associated with any pictures.";
	rdfs:label "No-Depiction".
	
:No-Employment a :Restriction;
	rdfs:comment "The no-employment restriction states that the owner of this profile does not want the information on this profile used for employment purposes.";
	rdfs:label "No-Employment".	

:No-Financial a :Restriction;
	rdfs:comment "The no-financial restriction states that the owner of this profile does not want the information on this profile used for financial decisions.";
	rdfs:label "No-Financial".	
	
:No-Medical a :Restriction;
	rdfs:comment "The no-medical restriction states that the owner of this profile does not want the information on this profile used for decisions related to medicine or medical care";
	rdfs:label "No-Medical".	
	
:No-Insurance a :Restriction;
	rdfs:comment "The no-insurance restriction states that the owner of this profile does not want the information on this profile used for decisions related for Insurance purposes";
	rdfs:label "No-Insurance".	

:Purpose a rdfs:Class;
	rdfs:comment "purpose";
	rdfs:label "Purpose or Use of data".

:use a rdfs:Property;
	rdfs:comment "Purpose of data";
	rdfs:label "purpose";
	rdfs:range :Purpose.

:cannot-be-used-for a rdfs:Property;
	rdfs:comment "Not an allowed purpose of data";
	rdfs:label "unallowed purpose";
	rdfs:range :Purpose.

:Commercial a :Purpose;
        rdfs:label "Commercial";
        owl:differentFrom :No-Commercial.

:Depiction a :Purpose;
        rdfs:label "Depiction";
        owl:differentFrom :No-Depiction.

:Employment a :Purpose;
        rdfs:label "Employment";
        owl:differentFrom :No-Employment.

:Financial a :Purpose;
        rdfs:label "Financial";
        owl:differentFrom :No-Financial.

:Medical a :Purpose;
        rdfs:label "Medical";
        owl:differentFrom :No-Medical.

:Insurance a :Purpose;
        rdfs:label "Medical";
        owl:differentFrom :No-Insurance.

# adding info for CC licenses because rdfa extraction isn't supported in Tabulator

:restricts rdfs:subPropertyOf cc:license.

<http://creativecommons.org/licenses/by-sa/3.0/> a cc:License;
	rdfs:label "CC:Attribution-ShareAlike".
<http://creativecommons.org/licenses/by/3.0/> a cc:License;
	rdfs:label "CC:Attribution".
<http://creativecommons.org/licenses/by-nd/3.0/> a cc:License;
	rdfs:label "CC:Attribution-NoDerivs".
<http://creativecommons.org/licenses/by-nc-nd/3.0/> a cc:License;
	rdfs:label "CC:Attribution-NonCommercial-NoDerivs".
<http://creativecommons.org/licenses/by-nc/3.0/> a cc:License;
	rdfs:label "CC:Attribution-NonCommercial".
<http://creativecommons.org/licenses/by-nc-sa/3.0/> a cc:License;
	rdfs:label "CC:Attribution-NonCommercial-ShareAlike".

<http://creativecommons.org/licenses/by-sa/3.0/us/> a cc:License;
        rdfs:label "CC:Attribution-ShareAlike".
<http://creativecommons.org/licenses/by/3.0/us/> a cc:License;
        rdfs:label "CC:Attribution".
<http://creativecommons.org/licenses/by-nd/3.0/us/> a cc:License;
        rdfs:label "CC:Attribution-NoDerivs".
<http://creativecommons.org/licenses/by-nc-nd/3.0/us/> a cc:License;
        rdfs:label "CC:Attribution-NonCommercial-NoDerivs".
<http://creativecommons.org/licenses/by-nc/3.0/us/> a cc:License;
        rdfs:label "CC:Attribution-NonCommercial".
<http://creativecommons.org/licenses/by-nc-sa/3.0/us/> a cc:License;
        rdfs:label "CC:Attribution-NonCommercial-ShareAlike".

#ends

